\documentclass{article}
\usepackage{epsfig}
\pagestyle{empty}
\begin{document}
$ R^{+} \times SO3 $
\pagebreak

$ s\cdot R $
\pagebreak

$ R $
\pagebreak

$ det(R)=1 $
\pagebreak

$ s>0 $
\pagebreak

$ Ad $
\pagebreak

$ A $
\pagebreak

$ x $
\pagebreak

$ \widehat{Ad_A\cdot x} = A\widehat{x}A^{-1} $
\pagebreak

$\ \widehat{\cdot} $
\pagebreak

$ sR $
\pagebreak

$ det(sR)=s^3 $
\pagebreak

$ \mathbf{R}^3 $
\pagebreak

$p \in \mathbf{R}^3 $
\pagebreak

$p' \in \mathbf{R}^3 $
\pagebreak

$p$
\pagebreak

$ p $
\pagebreak

$sR$
\pagebreak

$ p' = sR\cdot p $
\pagebreak

$ \frac{\partial}{\partial a} [a, b]_{rxso3} $
\pagebreak

$ [a, b]_{rxso3} $
\pagebreak

$ \omega $
\pagebreak

$ \exp(\widehat{a}) $
\pagebreak

$ \exp(\cdot) $
\pagebreak

$ \widehat{\cdot} $
\pagebreak

$ \theta = |\omega| $
\pagebreak

$ i \in \{0,1,2,3\} $
\pagebreak

$ i $
\pagebreak

$ G_i $
\pagebreak

$ G_0 = \left( \begin{array}{ccc} 0& 0& 0& \\ 0& 0& -1& \\ 0& 1& 0& \end{array} \right), G_1 = \left( \begin{array}{ccc} 0& 0& 1& \\ 0& 0& 0& \\ -1& 0& 0& \end{array} \right), G_2 = \left( \begin{array}{ccc} 0& -1& 0& \\ 1& 0& 0& \\ 0& 0& 0& \end{array} \right), G_3 = \left( \begin{array}{ccc} 1& 0& 0& \\ 0& 1& 0& \\ 0& 0& 1& \end{array} \right). $
\pagebreak

$ \widehat{\cdot}: \mathbf{R}^4 \rightarrow \mathbf{R}^{3\times 3}, \quad \widehat{a} = \sum_{i=0}^3 G_i a_i $
\pagebreak

$ [a, 2]_{rxso3} := [\widehat{a}, \widehat{b}]^\vee $
\pagebreak

$ [A,B] = AB-BA $
\pagebreak

$ (\cdot)^\vee $
\pagebreak

$ \log({\cdot})^\vee $
\pagebreak

$ \vee(\cdot) $
\pagebreak

$ \vee{\cdot} $
\pagebreak

$ \mathbf{R}^2 $
\pagebreak

$p \in \mathbf{R}^2 $
\pagebreak

$p' \in \mathbf{R}^2 $
\pagebreak

$R,t$
\pagebreak

$ p' = R\cdot p + t $
\pagebreak

$ \frac{\partial}{\partial a} [a, b]_{se2} $
\pagebreak

$ [a, b]_{se2} $
\pagebreak

$ a $
\pagebreak

$ \upsilon $
\pagebreak

$ \theta $
\pagebreak

$ i \in \{0,1,2\} $
\pagebreak

\[ G_0 = \left( \begin{array}{ccc} 0& 0& 1\\ 0& 0& 0\\ 0& 0& 0\\ \end{array} \right), G_1 = \left( \begin{array}{cccc} 0& 0& 0\\ 0& 0& 1\\ 0& 0& 0\\ \end{array} \right), G_2 = \left( \begin{array}{cccc} 0& 0& 0&\\ 0& 0& -1&\\ 0& 1& 0&\\ \end{array} \right), \]
\pagebreak

$ \widehat{\cdot}: \mathbf{R}^3 \rightarrow \mathbf{R}^{2\times 2}, \quad \widehat{\omega} = \sum_{i=0}^2 G_i \omega_i $
\pagebreak

$ [a, b]_{se2} := [\widehat{a_1}, \widehat{b_2}]^\vee $
\pagebreak

$ \frac{\partial}{\partial a} [a, b]_{se3} $
\pagebreak

$ [a, b]_{se3} $
\pagebreak

$ i \in \{0,1,2,3,4,5\} $
\pagebreak

\[ G_0 = \left( \begin{array}{cccc} 0& 0& 0& 1\\ 0& 0& 0& 0\\ 0& 0& 0& 0\\ 0& 0& 0& 0\\ \end{array} \right), G_1 = \left( \begin{array}{cccc} 0& 0& 0& 0\\ 0& 0& 0& 1\\ 0& 0& 0& 0\\ 0& 0& 0& 0\\ \end{array} \right), G_2 = \left( \begin{array}{cccc} 0& 0& 0& 0\\ 0& 0& 0& 0\\ 0& 0& 0& 1\\ 0& 0& 0& 0\\ \end{array} \right). G_3 = \left( \begin{array}{cccc} 0& 0& 0& 0\\ 0& 0& -1& 0\\ 0& 1& 0& 0\\ 0& 0& 0& 0\\ \end{array} \right), G_4 = \left( \begin{array}{cccc} 0& 0& 1& 0\\ 0& 0& 0& 0\\ -1& 0& 0& 0\\ 0& 0& 0& 0\\ \end{array} \right), G_5 = \left( \begin{array}{cccc} 0& -1& 0& 0\\ 1& 0& 0& 0\\ 0& 0& 0& 0\\ 0& 0& 0& 0\\ \end{array} \right). \]
\pagebreak

$ \widehat{\cdot}: \mathbf{R}^6 \rightarrow \mathbf{R}^{4\times 4}, \quad \widehat{\omega} = \sum_{i=0}^5 G_i \omega_i $
\pagebreak

$ [a, b]_{se3} := [\widehat{a}, \widehat{b}]^\vee $
\pagebreak

$sR,t$
\pagebreak

$ p' = sR\cdot p + t $
\pagebreak

$ \frac{\partial}{\partial a} [a, b]_{sim3} $
\pagebreak

$ [a, b]_{sim3} $
\pagebreak

$ i \in \{0,1,2,3,4,5,6\} $
\pagebreak

\[ G_0 = \left( \begin{array}{cccc} 0& 0& 0& 1\\ 0& 0& 0& 0\\ 0& 0& 0& 0\\ 0& 0& 0& 0\\ \end{array} \right), G_1 = \left( \begin{array}{cccc} 0& 0& 0& 0\\ 0& 0& 0& 1\\ 0& 0& 0& 0\\ 0& 0& 0& 0\\ \end{array} \right), G_2 = \left( \begin{array}{cccc} 0& 0& 0& 0\\ 0& 0& 0& 0\\ 0& 0& 0& 1\\ 0& 0& 0& 0\\ \end{array} \right). G_3 = \left( \begin{array}{cccc} 0& 0& 0& 0\\ 0& 0& -1& 0\\ 0& 1& 0& 0\\ 0& 0& 0& 0\\ \end{array} \right), G_4 = \left( \begin{array}{cccc} 0& 0& 1& 0\\ 0& 0& 0& 0\\ -1& 0& 0& 0\\ 0& 0& 0& 0\\ \end{array} \right), G_5 = \left( \begin{array}{cccc} 0& -1& 0& 0\\ 1& 0& 0& 0\\ 0& 0& 0& 0\\ 0& 0& 0& 0\\ \end{array} \right), G_6 = \left( \begin{array}{cccc} 1& 0& 0& 0\\ 0& 1& 0& 0\\ 0& 0& 1& 0\\ 0& 0& 0& 0\\ \end{array} \right). \]
\pagebreak

$ \widehat{\cdot}: \mathbf{R}^7 \rightarrow \mathbf{R}^{4\times 4}, \quad \widehat{\omega} = \sum_{i=0}^5 G_i \omega_i $
\pagebreak

$ [a, b]_{sim3} := [\widehat{a}, \widehat{b}]^\vee $
\pagebreak

$R$
\pagebreak

$ p' = R\cdot p $
\pagebreak

$ \exp(\widehat{\theta}) $
\pagebreak

$ G_0 = \left( \begin{array}{ccc} 0& -1& \\ 1& 0& \end{array} \right). $
\pagebreak

$ \widehat{\cdot}: \mathbf{R}^2 \rightarrow \mathbf{R}^{2\times 2}, \quad \widehat{\theta} = G_0\cdot \theta $
\pagebreak

$ G_0 $
\pagebreak

$ [\theta_1, \theta_2]_{so2} = 0 $
\pagebreak

$q$
\pagebreak

$ p' = q\cdot p \cdot q^{*} $
\pagebreak

$ q^{*} $
\pagebreak

$ q $
\pagebreak

$|\omega|$
\pagebreak

$\frac{\omega}{|\omega|}$
\pagebreak

$ \omega = \log(R)^\vee $
\pagebreak

$ \frac{\partial}{\partial a} [a, b]_{so3} $
\pagebreak

$ [a, b]_{so3} $
\pagebreak

$ \exp(\widehat{\omega}) $
\pagebreak

$ G_0 = \left( \begin{array}{ccc} 0& 0& 0& \\ 0& 0& -1& \\ 0& 1& 0& \end{array} \right), G_1 = \left( \begin{array}{ccc} 0& 0& 1& \\ 0& 0& 0& \\ -1& 0& 0& \end{array} \right), G_2 = \left( \begin{array}{ccc} 0& -1& 0& \\ 1& 0& 0& \\ 0& 0& 0& \end{array} \right). $
\pagebreak

$ \widehat{\cdot}: \mathbf{R}^3 \rightarrow \mathbf{R}^{3\times 3}, \quad \widehat{\omega} = \sum_{i=0}^2 G_i \omega_i $
\pagebreak

$ [\omega_1, \omega_2]_{so3} := [\widehat{\omega_1}, \widehat{\omega_2}]^\vee $
\pagebreak

$ [\omega_1, \omega_2]_{so3} = \omega_1 \times \omega_2 $
\pagebreak

$ R=\exp\left(\begin{array}{c}\alpha_1\\ 0\\ 0\end{array}\right) \cdot \exp\left(\begin{array}{c}0\\ \alpha_2\\ 0\end{array}\right) \cdot \exp\left(\begin{array}{c}0\\ 0\\ \alpha_3\end{array}\right)$
\pagebreak

\end{document}
